Let stateful tactics try all decompositions.
This problem has been reported by Léon Gondelman.

Before, when using, for example wp_alloc, in an expression like:

  ref (ref v)

It would apply `tac_wp_alloc` to the outermost ref, after which it
fails to establish that the argument `ref v` is a value. In this
commit, other evaluation positions will be tried whenever it turn
out that the argument of the construct is not a value. The same
applies to store/cas/...

I have implemented this by making use of the new `IntoVal` class.

theories/tests/heap_lang.v
@@ -42,6 +42,16 @@ Section LiftingTests.
     by repeat (wp_pure _).
   Qed.
 
+  Definition heap_e4 : expr :=
+    let: "x" := (let: "y" := ref (ref #1) in ref "y") in
+    ! ! !"x".
+
+  Lemma heap_e4_spec : WP heap_e4 {{ v, ⌜ v = #1 ⌝ }}%I.
+  Proof.
+    rewrite /heap_e4. wp_alloc l. wp_alloc l'. wp_let.
+    wp_alloc l''. wp_let. by repeat wp_load.
+  Qed.
+
   Definition FindPred : val :=
     rec: "pred" "x" "y" :=
       let: "yp" := "y" + #1 in
